Veir/IR/GetSet.lean
@@ -51,132 +51,135 @@ setup_grind_with_get_set_definitions
 
 /- OperationPtr.allocEmpty -/
 
-@[simp, grind =>]
-theorem BlockPtr.get!_OperationPtr_allocEmpty {block : BlockPtr}
-    (heq : OperationPtr.allocEmpty ctx ty properties = some (ctx', op')) :
-    block.get! ctx' = block.get! ctx := by
+@[simp, grind =]
+theorem BlockPtr.get!_OperationPtr_allocEmpty {block : BlockPtr} :
+  block.get! (OperationPtr.allocEmpty ctx ty properties).1 = block.get! ctx := by
   grind
 
-@[grind =>]
-theorem OperationPtr.get!_OperationPtr_allocEmpty {operation : OperationPtr}
-    (heq : OperationPtr.allocEmpty ctx ty properties = some (ctx', op')) :
-    operation.get! ctx' =
-    if operation = op' then Operation.empty ty properties else operation.get! ctx := by
+@[grind =]
+theorem OperationPtr.get!_OperationPtr_allocEmpty {operation : OperationPtr} :
+    operation.get! (OperationPtr.allocEmpty ctx ty properties).1 =
+    if operation = (OperationPtr.allocEmpty ctx ty properties).2 then
+      Operation.empty ty properties
+    else
+      operation.get! ctx := by
   grind
 
-@[grind =>]
-theorem OperationPtr.getOpType!_OperationPtr_allocEmpty {operation : OperationPtr}
-    (heq : OperationPtr.allocEmpty ctx ty properties = some (ctx', op')) :
-    operation.getOpType! ctx' =
-    if operation = op' then ty else operation.getOpType! ctx := by
+@[grind =]
+theorem OperationPtr.getOpType!_OperationPtr_allocEmpty {operation : OperationPtr} :
+    operation.getOpType! (OperationPtr.allocEmpty ctx ty properties).1 =
+    if operation = (OperationPtr.allocEmpty ctx ty properties).2 then
+      ty
+    else
+      operation.getOpType! ctx := by
   grind
 
-@[grind =>]
-theorem OperationPtr.getNumResults!_OperationPtr_allocEmpty {operation : OperationPtr}
-    (heq : OperationPtr.allocEmpty ctx ty properties = some (ctx', op')) :
-    operation.getNumResults! ctx' =
-    if operation = op' then 0 else operation.getNumResults! ctx := by
+@[grind =]
+theorem OperationPtr.getNumResults!_OperationPtr_allocEmpty {operation : OperationPtr} :
+    operation.getNumResults! (OperationPtr.allocEmpty ctx ty properties).1 =
+    if operation = (OperationPtr.allocEmpty ctx ty properties).2 then
+      0
+    else
+      operation.getNumResults! ctx := by
   grind
 
-@[grind =>]
-theorem OpResultPtr.get!_OperationPtr_allocEmpty {opResult : OpResultPtr}
-    (heq : OperationPtr.allocEmpty ctx ty properties = some (ctx', op')) :
-    opResult.get! ctx' = opResult.get! ctx := by
+@[grind =]
+theorem OpResultPtr.get!_OperationPtr_allocEmpty {opResult : OpResultPtr} :
+  opResult.get! (OperationPtr.allocEmpty ctx ty properties).1 = opResult.get! ctx := by
+  have := ctx.nextID_free
   grind [Operation.default_results_eq]
 
-@[grind =>]
-theorem OperationPtr.getNumOperands!_OperationPtr_allocEmpty {operation : OperationPtr}
-    (heq : OperationPtr.allocEmpty ctx ty properties = some (ctx', op')) :
-    operation.getNumOperands! ctx' =
-    if operation = op' then 0 else operation.getNumOperands! ctx := by
+@[grind =]
+theorem OperationPtr.getNumOperands!_OperationPtr_allocEmpty {operation : OperationPtr} :
+    operation.getNumOperands! (OperationPtr.allocEmpty ctx ty properties).1 =
+    if operation = (OperationPtr.allocEmpty ctx ty properties).2 then
+      0
+    else
+      operation.getNumOperands! ctx := by
   grind
 
-@[simp, grind =>]
-theorem OpOperandPtr.get!_OperationPtr_allocEmpty  {opOperand : OpOperandPtr}
-    (heq : OperationPtr.allocEmpty ctx ty properties = some (ctx', op')) :
-    opOperand.get! ctx' = opOperand.get! ctx := by
+@[simp, grind =]
+theorem OpOperandPtr.get!_OperationPtr_allocEmpty  {opOperand : OpOperandPtr} :
+  opOperand.get! (OperationPtr.allocEmpty ctx ty properties).1 = opOperand.get! ctx := by
+  have := ctx.nextID_free
   grind [Operation.default_operands_eq]
 
-@[simp, grind =>]
-theorem OperationPtr.getProperties!_OperationPtr_allocEmpty {operation : OperationPtr}
-    (heq : OperationPtr.allocEmpty ctx ty properties = some (ctx', op')) :
-    operation.getProperties! ctx' ty =
-    if operation = op' then properties else operation.getProperties! ctx ty := by
+@[simp, grind =]
+theorem OperationPtr.getProperties!_OperationPtr_allocEmpty {operation : OperationPtr} :
+    operation.getProperties! (OperationPtr.allocEmpty ctx ty properties).1 ty =
+    if operation = (OperationPtr.allocEmpty ctx ty properties).2 then
+      properties
+    else
+      operation.getProperties! ctx ty := by
   grind
 
-@[grind =>]
-theorem OperationPtr.getOperands!_OperationPtr_allocEmpty {operation : OperationPtr}
-    (heq : OperationPtr.allocEmpty ctx ty properties = some (ctx', op')) :
-    operation.getOperands! ctx' =
-    if operation = op' then #[] else operation.getOperands! ctx := by
+@[grind =]
+theorem OperationPtr.getOperands!_OperationPtr_allocEmpty {operation : OperationPtr} :
+    operation.getOperands! (OperationPtr.allocEmpty ctx ty properties).1 =
+    if operation = (OperationPtr.allocEmpty ctx ty properties).2 then
+      #[]
+    else
+      operation.getOperands! ctx := by
   grind
 
-@[grind =>]
-theorem OperationPtr.getNumSuccessors!_OperationPtr_allocEmpty {operation : OperationPtr}
-    (heq : OperationPtr.allocEmpty ctx ty properties = some (ctx', op')) :
-    operation.getNumSuccessors! ctx' =
-    if operation = op' then 0 else operation.getNumSuccessors! ctx := by
+@[grind =]
+theorem OperationPtr.getNumSuccessors!_OperationPtr_allocEmpty {operation : OperationPtr} :
+    operation.getNumSuccessors! (OperationPtr.allocEmpty ctx ty properties).1 =
+    if operation = (OperationPtr.allocEmpty ctx ty properties).2 then 0 else operation.getNumSuccessors! ctx := by
   grind
 
-@[simp, grind =>]
-theorem BlockOperandPtr.get!_OperationPtr_allocEmpty {blockOperand : BlockOperandPtr}
-    (heq : OperationPtr.allocEmpty ctx ty properties = some (ctx', op')) :
-    blockOperand.get! ctx' = blockOperand.get! ctx := by
+@[simp, grind =]
+theorem BlockOperandPtr.get!_OperationPtr_allocEmpty {blockOperand : BlockOperandPtr} :
+    blockOperand.get! (OperationPtr.allocEmpty ctx ty properties).1 = blockOperand.get! ctx := by
+  have := ctx.nextID_free
   grind [Operation.default_blockOperands_eq]
 
-@[grind =>]
-theorem OperationPtr.getNumRegions!_OperationPtr_allocEmpty {operation : OperationPtr}
-    (heq : OperationPtr.allocEmpty ctx ty properties = some (ctx', op')) :
-    operation.getNumRegions! ctx' =
-    if operation = op' then 0 else operation.getNumRegions! ctx := by
+@[grind =]
+theorem OperationPtr.getNumRegions!_OperationPtr_allocEmpty {operation : OperationPtr} :
+    operation.getNumRegions! (OperationPtr.allocEmpty ctx ty properties).1 =
+    if operation = (OperationPtr.allocEmpty ctx ty properties).2 then 0 else operation.getNumRegions! ctx := by
   grind
 
-@[simp, grind =>]
-theorem OperationPtr.getRegion!_OperationPtr_allocEmpty  {operation : OperationPtr}
-    (heq : OperationPtr.allocEmpty ctx ty properties = some (ctx', op')) :
-    operation.getRegion! ctx' i = operation.getRegion! ctx i := by
+@[simp, grind =]
+theorem OperationPtr.getRegion!_OperationPtr_allocEmpty  {operation : OperationPtr} :
+    operation.getRegion! (OperationPtr.allocEmpty ctx ty properties).1 i =
+    operation.getRegion! ctx i := by
+  have := ctx.nextID_free
   grind [Operation.default_regions_eq]
 
-@[simp, grind =>]
-theorem BlockOperandPtrPtr.get!_OperationPtr_allocEmpty {blockOperandPtr : BlockOperandPtrPtr}
-    (heq : OperationPtr.allocEmpty ctx ty properties = some (ctx', op')) :
-    blockOperandPtr.get! ctx' = blockOperandPtr.get! ctx := by
+@[simp, grind =]
+theorem BlockOperandPtrPtr.get!_OperationPtr_allocEmpty {blockOperandPtr : BlockOperandPtrPtr} :
+    blockOperandPtr.get! (OperationPtr.allocEmpty ctx ty properties).1 = blockOperandPtr.get! ctx := by
   grind
 
-@[simp, grind =>]
-theorem BlockPtr.getNumArguments!_OperationPtr_allocEmpty {block : BlockPtr}
-    (heq : OperationPtr.allocEmpty ctx ty properties = some (ctx', op')) :
-    block.getNumArguments! ctx' = block.getNumArguments! ctx := by
+@[simp, grind =]
+theorem BlockPtr.getNumArguments!_OperationPtr_allocEmpty {block : BlockPtr} :
+    block.getNumArguments! (OperationPtr.allocEmpty ctx ty properties).1 = block.getNumArguments! ctx := by
   grind
 
-@[simp, grind =>]
-theorem BlockArgumentPtr.get!_OperationPtr_allocEmpty {blockArg : BlockArgumentPtr}
-    (heq : OperationPtr.allocEmpty ctx ty properties = some (ctx', op')) :
-    blockArg.get! ctx' = blockArg.get! ctx := by
+@[simp, grind =]
+theorem BlockArgumentPtr.get!_OperationPtr_allocEmpty {blockArg : BlockArgumentPtr} :
+    blockArg.get! (OperationPtr.allocEmpty ctx ty properties).1 = blockArg.get! ctx := by
   grind
 
-@[simp, grind =>]
-theorem RegionPtr.get!_OperationPtr_allocEmpty {region : RegionPtr}
-    (heq : OperationPtr.allocEmpty ctx ty properties = some (ctx', op')) :
-    region.get! ctx' = region.get! ctx := by
+@[simp, grind =]
+theorem RegionPtr.get!_OperationPtr_allocEmpty {region : RegionPtr} :
+    region.get! (OperationPtr.allocEmpty ctx ty properties).1 = region.get! ctx := by
   grind
 
-@[simp, grind =>]
-theorem ValuePtr.getFirstUse!_OperationPtr_allocEmpty {value : ValuePtr}
-    (heq : OperationPtr.allocEmpty ctx ty properties = some (ctx', op')) :
-    value.getFirstUse! ctx' = value.getFirstUse! ctx := by
+@[simp, grind =]
+theorem ValuePtr.getFirstUse!_OperationPtr_allocEmpty {value : ValuePtr} :
+  value.getFirstUse! (OperationPtr.allocEmpty ctx ty properties).1 = value.getFirstUse! ctx := by
   grind
 
-@[simp, grind =>]
-theorem ValuePtr.getType!_OperationPtr_allocEmpty {value : ValuePtr}
-    (h : OperationPtr.allocEmpty ctx ty properties = some (ctx', op')) :
-    value.getType! ctx' = value.getType! ctx := by
+@[simp, grind =]
+theorem ValuePtr.getType!_OperationPtr_allocEmpty {value : ValuePtr} :
+  value.getType! (OperationPtr.allocEmpty ctx ty properties).1 = value.getType! ctx := by
   grind
 
-@[simp, grind =>]
-theorem OpOperandPtrPtr.get!_OperationPtr_allocEmpty {opOperandPtr : OpOperandPtrPtr}
-    (heq : OperationPtr.allocEmpty ctx ty properties = some (ctx', op')) :
-    opOperandPtr.get! ctx' = opOperandPtr.get! ctx := by
+@[simp, grind =]
+theorem OpOperandPtrPtr.get!_OperationPtr_allocEmpty {opOperandPtr : OpOperandPtrPtr} :
+  opOperandPtr.get! (OperationPtr.allocEmpty ctx ty properties).1 = opOperandPtr.get! ctx := by
   grind
 
 /- OperationPtr.dealloc -/
@@ -2443,116 +2446,117 @@ theorem OpOperandPtrPtr.get!_BlockArgumentPtr_setLoc {opOperandPtr : OpOperandPt
 
 @[grind =>]
 theorem BlockPtr.get!_BlockPtr_allocEmpty {block : BlockPtr}
-    (heq : BlockPtr.allocEmpty ctx = some (ctx', bl')) :
+    (heq : BlockPtr.allocEmpty ctx = (ctx', bl')) :
     block.get! ctx' = if block = bl' then Block.empty else block.get! ctx := by
   grind
 
 @[simp, grind =>]
 theorem OperationPtr.get!_BlockPtr_allocEmpty {operation : OperationPtr}
-    (heq : BlockPtr.allocEmpty ctx = some (ctx', bl)) :
+    (heq : BlockPtr.allocEmpty ctx = (ctx', bl)) :
     operation.get! ctx' = operation.get! ctx := by
   grind
 
 @[simp, grind =>]
 theorem OperationPtr.getOpType!_BlockPtr_allocEmpty {operation : OperationPtr}
-    (heq : BlockPtr.allocEmpty ctx = some (ctx', bl)) :
+    (heq : BlockPtr.allocEmpty ctx = (ctx', bl)) :
     operation.getOpType! ctx' = operation.getOpType! ctx := by
   grind
 
 @[simp, grind =>]
 theorem OperationPtr.getProperties!_BlockPtr_allocEmpty {operation : OperationPtr}
-    (heq : BlockPtr.allocEmpty ctx = some (ctx', bl)) :
+    (heq : BlockPtr.allocEmpty ctx = (ctx', bl)) :
     operation.getProperties! ctx' opCode = operation.getProperties! ctx opCode := by
   grind
 
 @[simp, grind =>]
 theorem OperationPtr.getNumResults!_BlockPtr_allocEmpty {operation : OperationPtr}
-    (heq : BlockPtr.allocEmpty ctx = some (ctx', bl)) :
+    (heq : BlockPtr.allocEmpty ctx = (ctx', bl)) :
     operation.getNumResults! ctx' = operation.getNumResults! ctx := by
   grind
 
 @[simp, grind =>]
 theorem OpResultPtr.get!_BlockPtr_allocEmpty {opResult : OpResultPtr}
-    (heq : BlockPtr.allocEmpty ctx = some (ctx', bl')) :
+    (heq : BlockPtr.allocEmpty ctx = (ctx', bl')) :
     opResult.get! ctx' = opResult.get! ctx := by
   grind
 
 @[simp, grind =>]
 theorem OperationPtr.getNumOperands!_BlockPtr_allocEmpty {operation : OperationPtr}
-    (heq : BlockPtr.allocEmpty ctx = some (ctx', bl)) :
+    (heq : BlockPtr.allocEmpty ctx = (ctx', bl)) :
     operation.getNumOperands! ctx' = operation.getNumOperands! ctx := by
   grind
 
 @[simp, grind =>]
 theorem OpOperandPtr.get!_BlockPtr_allocEmpty  {opOperand : OpOperandPtr}
-    (heq : BlockPtr.allocEmpty ctx = some (ctx', bl')) :
+    (heq : BlockPtr.allocEmpty ctx = (ctx', bl')) :
     opOperand.get! ctx' = opOperand.get! ctx := by
   grind
 
 @[simp, grind =>]
 theorem OperationPtr.getOperands!_BlockPtr_allocEmpty {operation : OperationPtr}
-    (heq : BlockPtr.allocEmpty ctx = some (ctx', bl)) :
+    (heq : BlockPtr.allocEmpty ctx = (ctx', bl)) :
     operation.getOperands! ctx' = operation.getOperands! ctx := by
   grind
 
 @[simp, grind =>]
 theorem OperationPtr.getNumSuccessors!_BlockPtr_allocEmpty {operation : OperationPtr}
-    (heq : BlockPtr.allocEmpty ctx = some (ctx', bl)) :
+    (heq : BlockPtr.allocEmpty ctx = (ctx', bl)) :
     operation.getNumSuccessors! ctx' = operation.getNumSuccessors! ctx := by
   grind
 
 @[simp, grind =>]
 theorem BlockOperandPtr.get!_BlockPtr_allocEmpty {blockOperand : BlockOperandPtr}
-    (heq : BlockPtr.allocEmpty ctx = some (ctx', bl')) :
+    (heq : BlockPtr.allocEmpty ctx = (ctx', bl')) :
     blockOperand.get! ctx' = blockOperand.get! ctx := by
   grind
 
 @[simp, grind =>]
 theorem OperationPtr.getNumRegions!_BlockPtr_allocEmpty {operation : OperationPtr}
-    (heq : BlockPtr.allocEmpty ctx = some (ctx', bl')) :
+    (heq : BlockPtr.allocEmpty ctx = (ctx', bl')) :
     operation.getNumRegions! ctx' = operation.getNumRegions! ctx := by
   grind
 
 @[simp, grind =>]
 theorem OperationPtr.getRegion!_BlockPtr_allocEmpty {operation : OperationPtr}
-    (heq : BlockPtr.allocEmpty ctx = some (ctx', bl')) :
+    (heq : BlockPtr.allocEmpty ctx = (ctx', bl')) :
     operation.getRegion! ctx' i = operation.getRegion! ctx i := by
   grind
 
 @[simp, grind =>]
 theorem BlockPtr.getNumArguments!_BlockPtr_allocEmpty {block : BlockPtr}
-    (heq : BlockPtr.allocEmpty ctx = some (ctx', bl')) :
+    (heq : BlockPtr.allocEmpty ctx = (ctx', bl')) :
     block.getNumArguments! ctx' =
     if block = bl' then 0 else block.getNumArguments! ctx := by
   grind
 
 @[simp, grind =>]
 theorem BlockArgumentPtr.get!_BlockPtr_allocEmpty {blockArg : BlockArgumentPtr}
-    (heq : BlockPtr.allocEmpty ctx = some (ctx', bl')) :
+    (heq : BlockPtr.allocEmpty ctx = (ctx', bl')) :
     blockArg.get! ctx' = blockArg.get! ctx := by
+  have := ctx.nextID_free
   grind [Block.default_arguments_eq]
 
 @[simp, grind =>]
 theorem RegionPtr.get!_BlockPtr_allocEmpty {region : RegionPtr}
-    (heq : BlockPtr.allocEmpty ctx = some (ctx', bl')) :
+    (heq : BlockPtr.allocEmpty ctx = (ctx', bl')) :
     region.get! ctx' = region.get! ctx := by
   grind
 
 @[simp, grind =>]
 theorem ValuePtr.getFirstUse!_BlockPtr_allocEmpty {value : ValuePtr}
-    (heq : BlockPtr.allocEmpty ctx = some (ctx', bl')) :
+    (heq : BlockPtr.allocEmpty ctx = (ctx', bl')) :
     value.getFirstUse! ctx' = value.getFirstUse! ctx := by
   grind
 
  @[simp, grind =>]
 theorem ValuePtr.getType!_BlockPtr_allocEmpty {value : ValuePtr}
-    (heq : BlockPtr.allocEmpty ctx = some (ctx', bl')) :
+    (heq : BlockPtr.allocEmpty ctx = (ctx', bl')) :
     value.getType! ctx' = value.getType! ctx := by
   grind
 
 @[simp, grind =>]
 theorem OpOperandPtrPtr.get!_BlockPtr_allocEmpty {opOperandPtr : OpOperandPtrPtr}
-    (heq : BlockPtr.allocEmpty ctx = some (ctx', bl')) :
+    (heq : BlockPtr.allocEmpty ctx = (ctx', bl')) :
     opOperandPtr.get! ctx' = opOperandPtr.get! ctx := by
   grind
 
@@ -4499,121 +4503,121 @@ theorem OpOperandPtrPtr.get!_OpResultPtr_setFirstUse {opOperandPtr : OpOperandPt
 
 @[simp, grind =>]
 theorem BlockPtr.get!_RegionPtr_allocEmpty {block : BlockPtr}
-    (heq : RegionPtr.allocEmpty ctx = some (ctx', rg')) :
+    (heq : RegionPtr.allocEmpty ctx = (ctx', rg')) :
     block.get! ctx' = block.get! ctx := by
   grind
 
 @[grind =>]
 theorem OperationPtr.get!_RegionPtr_allocEmpty {operation : OperationPtr}
-    (heq : RegionPtr.allocEmpty ctx = some (ctx', rg')) :
+    (heq : RegionPtr.allocEmpty ctx = (ctx', rg')) :
     operation.get! ctx' = operation.get! ctx := by
   grind
 
 @[simp, grind =>]
 theorem OperationPtr.getOpType!_RegionPtr_allocEmpty {operation : OperationPtr}
-    (heq : RegionPtr.allocEmpty ctx = some (ctx', rg')) :
+    (heq : RegionPtr.allocEmpty ctx = (ctx', rg')) :
     operation.getOpType! ctx' = operation.getOpType! ctx := by
   grind
 
 @[grind =>]
 theorem OperationPtr.getProperties!_RegionPtr_allocEmpty {operation : OperationPtr}
-    (heq : RegionPtr.allocEmpty ctx = some (ctx', rg')) :
+    (heq : RegionPtr.allocEmpty ctx = (ctx', rg')) :
     operation.getProperties! ctx' opCode = operation.getProperties! ctx opCode := by
   grind
 
 @[grind =>]
 theorem OperationPtr.getNumResults!_RegionPtr_allocEmpty {operation : OperationPtr}
-    (heq : RegionPtr.allocEmpty ctx = some (ctx', rg')) :
+    (heq : RegionPtr.allocEmpty ctx = (ctx', rg')) :
     operation.getNumResults! ctx' = operation.getNumResults! ctx := by
   grind
 
 @[grind =>]
 theorem OpResultPtr.get!_RegionPtr_allocEmpty {opResult : OpResultPtr}
-    (heq : RegionPtr.allocEmpty ctx = some (ctx', rg')) :
+    (heq : RegionPtr.allocEmpty ctx = (ctx', rg')) :
     opResult.get! ctx' = opResult.get! ctx := by
   grind [Operation.default_results_eq]
 
 @[grind =>]
 theorem OperationPtr.getNumOperands!_RegionPtr_allocEmpty {operation : OperationPtr}
-    (heq : RegionPtr.allocEmpty ctx = some (ctx', rg')) :
+    (heq : RegionPtr.allocEmpty ctx = (ctx', rg')) :
     operation.getNumOperands! ctx' = operation.getNumOperands! ctx := by
   grind
 
 @[simp, grind =>]
 theorem OpOperandPtr.get!_RegionPtr_allocEmpty  {opOperand : OpOperandPtr}
-    (heq : RegionPtr.allocEmpty ctx = some (ctx', rg')) :
+    (heq : RegionPtr.allocEmpty ctx = (ctx', rg')) :
     opOperand.get! ctx' = opOperand.get! ctx := by
   grind [Operation.default_operands_eq]
 
 @[simp, grind =>]
 theorem OperationPtr.getOperands!_RegionPtr_allocEmpty {operation : OperationPtr}
-    (heq : RegionPtr.allocEmpty ctx = some (ctx', rg')) :
+    (heq : RegionPtr.allocEmpty ctx = (ctx', rg')) :
     operation.getOperands! ctx' = operation.getOperands! ctx := by
   grind
 
 @[grind =>]
 theorem OperationPtr.getNumSuccessors!_RegionPtr_allocEmpty {operation : OperationPtr}
-    (heq : RegionPtr.allocEmpty ctx = some (ctx', rg')) :
+    (heq : RegionPtr.allocEmpty ctx = (ctx', rg')) :
     operation.getNumSuccessors! ctx' = operation.getNumSuccessors! ctx := by
   grind
 
 @[simp, grind =>]
 theorem BlockOperandPtr.get!_RegionPtr_allocEmpty {blockOperand : BlockOperandPtr}
-    (heq : RegionPtr.allocEmpty ctx = some (ctx', rg')) :
+    (heq : RegionPtr.allocEmpty ctx = (ctx', rg')) :
     blockOperand.get! ctx' = blockOperand.get! ctx := by
   grind [Operation.default_blockOperands_eq]
 
 @[grind =>]
 theorem OperationPtr.getNumRegions!_RegionPtr_allocEmpty {operation : OperationPtr}
-    (heq : RegionPtr.allocEmpty ctx = some (ctx', rg')) :
+    (heq : RegionPtr.allocEmpty ctx = (ctx', rg')) :
     operation.getNumRegions! ctx' = operation.getNumRegions! ctx := by
   grind
 
 @[simp, grind =>]
 theorem OperationPtr.getRegion!_RegionPtr_allocEmpty  {operation : OperationPtr}
-    (heq : RegionPtr.allocEmpty ctx = some (ctx', rg')) :
+    (heq : RegionPtr.allocEmpty ctx = (ctx', rg')) :
     operation.getRegion! ctx' i = operation.getRegion! ctx i := by
   grind [Operation.default_regions_eq]
 
 @[simp, grind =>]
 theorem BlockOperandPtrPtr.get!_RegionPtr_allocEmpty {blockOperandPtr : BlockOperandPtrPtr}
-    (heq : RegionPtr.allocEmpty ctx = some (ctx', rg')) :
+    (heq : RegionPtr.allocEmpty ctx = (ctx', rg')) :
     blockOperandPtr.get! ctx' = blockOperandPtr.get! ctx := by
   grind
 
 @[simp, grind =>]
 theorem BlockPtr.getNumArguments!_RegionPtr_allocEmpty {block : BlockPtr}
-    (heq : RegionPtr.allocEmpty ctx = some (ctx', rg')) :
+    (heq : RegionPtr.allocEmpty ctx = (ctx', rg')) :
     block.getNumArguments! ctx' = block.getNumArguments! ctx := by
   grind
 
 @[simp, grind =>]
 theorem BlockArgumentPtr.get!_RegionPtr_allocEmpty {blockArg : BlockArgumentPtr}
-    (heq : RegionPtr.allocEmpty ctx = some (ctx', rg')) :
+    (heq : RegionPtr.allocEmpty ctx = (ctx', rg')) :
     blockArg.get! ctx' = blockArg.get! ctx := by
   grind
 
 @[simp, grind =>]
 theorem RegionPtr.get!_RegionPtr_allocEmpty {region : RegionPtr}
-    (heq : RegionPtr.allocEmpty ctx = some (ctx', rg')) :
+    (heq : RegionPtr.allocEmpty ctx = (ctx', rg')) :
     region.get! ctx' = if region = rg' then Region.empty else region.get! ctx := by
   grind
 
 @[simp, grind =>]
 theorem ValuePtr.getFirstUse!_RegionPtr_allocEmpty {value : ValuePtr}
-    (heq : RegionPtr.allocEmpty ctx = some (ctx', rg')) :
+    (heq : RegionPtr.allocEmpty ctx = (ctx', rg')) :
     value.getFirstUse! ctx' = value.getFirstUse! ctx := by
   grind
 
 @[simp, grind =>]
 theorem ValuePtr.getType!_RegionPtr_allocEmpty {value : ValuePtr}
-    (_ : RegionPtr.allocEmpty ctx = some (ctx', rg')) :
+    (_ : RegionPtr.allocEmpty ctx = (ctx', rg')) :
     value.getType! ctx' = value.getType! ctx := by
   grind
 
 @[simp, grind =>]
 theorem OpOperandPtrPtr.get!_RegionPtr_allocEmpty {opOperandPtr : OpOperandPtrPtr}
-    (heq : RegionPtr.allocEmpty ctx = some (ctx', rg')) :
+    (heq : RegionPtr.allocEmpty ctx = (ctx', rg')) :
     opOperandPtr.get! ctx' = opOperandPtr.get! ctx := by
   grind
 
